forward_call issue [skip ci]

src/Lib/DWT/VSTder_write_TL.v
@@ -10,8 +10,51 @@ Require Import Clight.dummy Lib.Callback.Dummy ExecBer_tlv_tag_serialize
 Require Import VSTber_tlv_length_serialize
         VSTber_tlv_tag_serialize.
 
-Definition Vprog : varspecs. mk_varspecs prog. Defined.
-Instance CompSpecs : compspecs. make_compspecs prog. Defined.
+Definition composites := composites ++ (match find_cs 
+                                            dummy._dummy
+                                            dummy.composites with
+                      | Some r => [r]
+                      | None => []
+                      end).
+
+Definition Vprog : varspecs. 
+Proof.
+  set (cs := composites).
+  set (gd := global_definitions).
+  set (pi := public_idents).
+  unfold composites in cs.
+  simpl in cs.
+  set (prog := Clightdefs.mkprogram cs gd pi _main Logic.I).
+  mk_varspecs prog. 
+Defined.
+
+Instance CompSpecs : compspecs. 
+Proof.
+  set (cs := composites).
+  set (gd := global_definitions).
+  set (pi := public_idents).
+  unfold composites in cs.
+  simpl in cs.
+  set (prog := Clightdefs.mkprogram cs gd pi _main Logic.I).
+  make_compspecs prog.
+Defined.
+
+(* Callback compspecs *)
+Instance Change3 : change_composite_env Dummy.CompSpecs CompSpecs.
+Proof. make_cs_preserve Dummy.CompSpecs CompSpecs. Defined.
+
+Instance Change4 : change_composite_env CompSpecs Dummy.CompSpecs.
+Proof. make_cs_preserve CompSpecs Dummy.CompSpecs. Defined.
+
+Instance Change5 : change_composite_env  VSTber_tlv_length_serialize.CompSpecs
+                                         VSTber_tlv_tag_serialize.CompSpecs.
+Proof. make_cs_preserve  VSTber_tlv_length_serialize.CompSpecs 
+       VSTber_tlv_tag_serialize.CompSpecs. Defined.
+
+Instance Change6: change_composite_env VSTber_tlv_tag_serialize.CompSpecs
+                                       VSTber_tlv_length_serialize.CompSpecs.
+Proof. make_cs_preserve VSTber_tlv_tag_serialize.CompSpecs
+                        VSTber_tlv_length_serialize.CompSpecs. Defined.
 
 Instance Change1 : change_composite_env CompSpecs  VSTber_tlv_tag_serialize.CompSpecs.
 Proof. make_cs_preserve CompSpecs  VSTber_tlv_tag_serialize.CompSpecs. Defined.
@@ -19,10 +62,10 @@ Proof. make_cs_preserve CompSpecs  VSTber_tlv_tag_serialize.CompSpecs. Defined.
 Instance Change2 : change_composite_env  VSTber_tlv_tag_serialize.CompSpecs CompSpecs.
 Proof. make_cs_preserve  VSTber_tlv_tag_serialize.CompSpecs CompSpecs. Defined.
 
-Instance Change3 : change_composite_env CompSpecs  VSTber_tlv_length_serialize.CompSpecs.
+Instance Change33 : change_composite_env CompSpecs  VSTber_tlv_length_serialize.CompSpecs.
 Proof. make_cs_preserve CompSpecs VSTber_tlv_length_serialize.CompSpecs. Defined.
 
-Instance Change4 : change_composite_env  VSTber_tlv_length_serialize.CompSpecs CompSpecs.
+Instance Change44 : change_composite_env  VSTber_tlv_length_serialize.CompSpecs CompSpecs.
 Proof. make_cs_preserve  VSTber_tlv_length_serialize.CompSpecs CompSpecs. Defined.
 
 Open Scope Z.
@@ -85,7 +128,9 @@ Definition der_write_TL_spec : ident * funspec :=
 
 Definition Gprog := ltac:(with_library prog [der_write_TL_spec;
                                              ber_tlv_tag_serialize_spec; 
-                                             der_tlv_length_serialize_spec]).
+                                             der_tlv_length_serialize_spec;
+                                             dummy_callback]).
+
 
 Open Scope Z.
 
@@ -94,6 +139,8 @@ Theorem der_write_TL_serialize_correct :
              der_write_TL_spec.
 Proof.
   start_function.
+  unfold MORE_COMMANDS.
+  unfold abbreviate.
   forward.
   unfold POSTCONDITION.
   forward_if 
@@ -173,9 +220,12 @@ Proof.
       discriminate.
     + (* cb <> nullval *)
       pose proof (tag_serialize_req_size tag (Int.repr 32)) as TT.
-      pose proof (tag_serialize_req_size len (Int.repr 32)) as LL.
+      pose proof (tag_serialize_req_size 
+                    len (Int.repr (32 - 
+                                   snd ((ber_tlv_tag_serialize tag (Int.repr 32)))))) as LL.
       break_let.
       break_let.
+      cbn in Heqp.
      pose proof (tag_serialize_bounds tag (Int.repr 32)) as TL.
      repeat forward.
      forward_call (tag, b, i, 32, 32).
@@ -274,6 +324,7 @@ Proof.
          ** 
            unfold POSTCONDITION.
            unfold abbreviate.
+           
            repeat break_let. 
            repeat forward.
            Exists (Vptr b i).
@@ -310,92 +361,101 @@ Proof.
            remember (snd (ber_tlv_tag_serialize tag (Int.repr 32))) as z0.
            remember (fst (ber_tlv_tag_serialize tag (Int.repr 32))) as ls.
            break_if. 
-           +++ assert (l2 = ls ++ l1) as L0.
-               { subst.
-                 replace l2 with (fst (der_write_TL tag len 32)).
-                 erewrite <- app_nil_end.
-                 unfold der_write_TL.
-                 repeat break_let.
-                 cbn in *.
-                 replace ((z0 =? -1) || (z0 >? 32))%bool with false.
-                 assert ((snd (ber_tlv_length_serialize len (Int.repr (32 - z0)))) = z3) as B.
-                 { unfold snd.
-                   break_let.
-                   auto.
-                   inversion Heqp4.
-                   auto. }
-                 assert (z3 = z1) as F.
-                 rewrite Heqp4 in Heqp1.
-                 inversion Heqp1. auto.
-                 pose proof (length_serialize_bounds len (Int.repr (32 - z0))) as L.
-                 assert (z3 = -1) as Z0. 
-                 { eapply repr_inj_signed;
-                     try rep_omega; subst; auto. }
-                 rewrite Z0.
-                 cbn.
-                 rewrite Heqp4 in Heqp1.
-                 inversion Heqp1.
-                  erewrite <- app_nil_end.
-                  auto.                  
-                 symmetry.
-                 eapply orb_false_intro;
-                   Zbool_to_Prop; try nia.
-                 erewrite Z.gtb_ltb.
-                 Zbool_to_Prop. nia.
-                 unfold fst.
+           +++ 
+             assert (l2 = ls ++ l1) as L0.
+             { subst.
+               replace l2 with (fst (der_write_TL tag len 32)).
+               erewrite <- app_nil_end.
+               unfold der_write_TL.
+               repeat break_let.
+               cbn in *.
+               replace ((z0 =? -1) || (z0 >? 32))%bool with false.
+               assert ((snd (ber_tlv_length_serialize len (Int.repr (32 - z0)))) = z3) as B.
+               { unfold snd.
                  break_let.
-                 congruence. }
-                 rewrite L0.
-                 erewrite sepcon_comm.
-                 erewrite <- data_at_app_gen.
-                 entailer!.
-                 admit. 
                  auto.
-                 {  subst; unfold default_val;
-                      simpl;
-                      try erewrite Zlength_list_repeat;
-                      try nia; auto. } 
-                 nia.
-                 rewrite <- Heqls.
-                 rewrite e.
-                 erewrite <- app_nil_end.
-                 erewrite Zlength_map in *.
-                 erewrite H4.
-                 autorewrite with sublist list norm.
-                 f_equal.
-                 unfold default_val.
-                   simpl.
-                   try erewrite Zlength_list_repeat.                   
-                 erewrite <- sublist_list_repeat with (k := 32).
-                 auto.
-                 all: try nia.
-                 setoid_rewrite H4.
-                 unfold tarray.
-                 erewrite Zlength_default_val_Tarray_tuchar.
-                 all: rep_omega.
+                 inversion Heqp4.
+                 auto. }
+               assert (z3 = z1) as F.
+               rewrite Heqp4 in Heqp1.
+               inversion Heqp1. auto.
+               pose proof (length_serialize_bounds len (Int.repr (32 - z0))) as L.
+               assert (z3 = -1) as Z0. 
+               { eapply repr_inj_signed;
+                   try rep_omega; subst; auto. }
+               rewrite Z0.
+               cbn.
+               rewrite Heqp4 in Heqp1.
+               inversion Heqp1.
+               erewrite <- app_nil_end.
+               auto.                  
+               symmetry.
+               eapply orb_false_intro;
+                 Zbool_to_Prop; try nia.
+               erewrite Z.gtb_ltb.
+               Zbool_to_Prop. nia.
+               unfold fst.
+               break_let.
+               congruence. }
+             rewrite L0.
+             erewrite sepcon_comm.
+             erewrite <- data_at_app_gen.
+             entailer!.
+             admit. 
+             auto.
+             {  subst; unfold default_val;
+                  simpl;
+                  try erewrite Zlength_list_repeat;
+                  try nia; auto. } 
+             nia.
+             rewrite <- Heqls.
+             rewrite e.
+             erewrite <- app_nil_end.
+             erewrite Zlength_map in *.
+             erewrite H4.
+             autorewrite with sublist list norm.
+             f_equal.
+             unfold default_val.
+             simpl.
+             try erewrite Zlength_list_repeat.                   
+             erewrite <- sublist_list_repeat with (k := 32).
+             auto.
+             all: try nia.
+             setoid_rewrite H4.
+             unfold tarray.
+             erewrite Zlength_default_val_Tarray_tuchar.
+             all: rep_omega.
            +++  admit. (* wrong data_at introduced automatically *)
          ** repeat forward.
             forward_if.
             ***
-              forward.
-              entailer!.
-              unfold der_write_TL.
+              unfold POSTCONDITION.
+              unfold abbreviate.
               repeat break_let.
+              clear Heqp.
+              forward.
+              Exists (Vptr b i).
+              entailer!.
+              replace z2 with (snd (der_write_TL tag len 32))
+                by (unfold snd; break_let; inversion Heqp2; auto).
+              unfold der_write_TL.
+              erewrite Heqp0.
+              erewrite Heqp1.
               cbn in *.
               do 2 f_equal.
-              replace ((z =? -1) || (z >? 32))%bool with false.
-              assert ((snd (ber_tlv_length_serialize len (Int.repr (32 - z)))) = z0) as B.
+                remember (snd (ber_tlv_tag_serialize tag (Int.repr 32))) as z0.
+                remember (fst (ber_tlv_tag_serialize tag (Int.repr 32))) as ls.
+                replace ((z0 =? -1) || (z0 >? 32))%bool with false.
+                assert ((snd (ber_tlv_length_serialize 
+                                len (Int.repr (32 - z0)))) = z1) as B.
               { unfold snd.
-                break_let.
-                auto.
-                inversion Heqp0.
-                auto. }
-              rewrite B in *.
-              pose proof (length_serialize_bounds len (Int.repr (32 - z))) as L.
-              assert (z0 <> -1) as Z0. 
+                rewrite Heqp1. auto. }
+             (* rewrite B in *. *)
+              pose proof (length_serialize_bounds len (Int.repr (32 - z0))) as L.
+              assert (z1 <> -1) as Z0. 
               { eapply repr_neq_e. auto. }
-              replace (z0 =? -1) with false.
-              replace (z0 + z >? 32) with true.
+              replace (z1 =? -1) with false.
+              replace (z1 + z0 >? 32) with true.
               auto.
               symmetry.
               erewrite Z.gtb_ltb.
@@ -408,14 +468,55 @@ Proof.
                 Zbool_to_Prop; try nia.
               erewrite Z.gtb_ltb.
               Zbool_to_Prop. nia.
-              remember (snd (ber_tlv_tag_serialize tag (Int.repr 32))) as z.
+              remember (snd (ber_tlv_tag_serialize tag (Int.repr 32))) as z0.
               remember (fst (ber_tlv_tag_serialize tag (Int.repr 32))) as ls.
-              break_let.
-              break_if. 
-              admit. (* fix SEP spec *)
-              admit.
+              break_if.
+              ---
+                erewrite sepcon_comm.
+                erewrite <- data_at_app_gen.
+                entailer!.
+                admit.
+                auto.
+                {  subst; unfold default_val;
+                  simpl;
+                  try erewrite Zlength_list_repeat;
+                  try nia; auto. } 
+                nia.
+                f_equal.
+                admit.
+                admit.
+                setoid_rewrite H5.
+             unfold tarray.
+             erewrite Zlength_default_val_Tarray_tuchar.
+             all: rep_omega.
+              ---
+                erewrite sepcon_comm.
+                (* erewrite <- data_at_app_gen. *)
+                admit.
             *** forward_if True; try congruence.
-        -- forward_if True.
+               -- normalize. forward_if True.
+                  replace z0 with (Notations.len (map Vint ls)).
+                  erewrite split_data_at_sublist_tuchar with (j := 1%Z).
+                  erewrite sublist_one.
+                  erewrite data_at_tuchar_singleton_array_eq.
+                  Intros.
+                  assert ((0 <= 0 < Notations.len ls)) by admit.
+                  forward.
+                  entailer!.
+                  admit.
+                  forward.
+                  replace (Notations.len (map Vint ls)) with z0.
+                  entailer!.
+                  remember (snd (ber_tlv_tag_serialize tag (Int.repr 32))) as z0.
+                  remember (fst (ber_tlv_tag_serialize tag (Int.repr 32))) as ls.
+                  normalize.
+                  1-8 : admit.
+                  forward.
+                  entailer!.
+                  hint.
+                  Intros.
+                  
+                  forward_call ((Vptr b i), z, app_key).
            ++
              (* store - add to spec *)
              admit.
