src/Lib/Callback/Dummy.v
@@ -8,7 +8,23 @@ Definition Vprog : varspecs. mk_varspecs prog. Defined.
 
 Open Scope Z.
 
-Definition dummy_callback_spec  : funspec :=
+ Definition dummy_callback_spec (z : Z)  : funspec :=
+    WITH data_p : val, size : Z,
+         key_p : val
+    PRE [tarray tuchar z, tuint, tptr tvoid]
+      PROP (0 <= size <= Int.max_unsigned)
+      PARAMS (data_p; Vint (Int.repr size); key_p)
+      GLOBALS ()
+      SEP ()
+    POST [tint]
+      PROP ()
+      LOCAL (temp ret_temp (if size =? 0 then (Vint (Int.repr (-1))) else Vzero))
+      SEP (). 
+
+Definition dummy_callback : ident * funspec :=
+  DECLARE _dummy dummy_callback_spec 32.
+
+(* Definition dummy_callback_spec  : funspec :=
     WITH data_p : val, size : Z,
          key_p : val
     PRE [tptr tvoid, tuint, tptr tvoid]
@@ -45,4 +61,4 @@ Proof.
     entailer!.
     break_if; [rewrite Z.eqb_eq in Heqb; congruence| reflexivity].
   * forward.
-Qed.
+Qed. *)
